$$\begin{align}
&\text{2a}\\
&\int(3+3\sqrt{ x })dx=3x+2x^{3/2}+C\\
&\text{b} \\
&\int(3-\cos x+3x^2)dx=3x-\sin x+x^3+C \\
&\text{d} \\
&\int \frac {}{} \\
&\text{2i} \\
&\int \frac{x^2+3x-2}{\sqrt{ x }}dx=\int(x^{3/2}+3x^{1/2}-2x^{-1/2})dx=\frac{2}{5}x^{5/2}+2x^{3/2}-4x^{1/2}+C \\
 \\
&\text{3a} \\
&\int \sec(2x-3)\tan(2x-3)dx \\
&=\frac{1}{2}\int \sec(2x-3)\tan(2x-3)d(2x-3) \\
&=\frac{1}{2}\sec(2x-3)+C \\
&\text{b} \\
&\int 2\cos^3{x} \sin{x} dx \\
 \\
&=\frac{-\cos^{4}x}{2} \\
&\text{3i} \\
&\int \sin 4x \cos 5x dx \\
&=\frac{1}{2}\int[\sin 9x-\sin x] dx \\
&=-\frac{1}{18} \cos 9x + \frac{1}{2}\cos x+C \\
&\text{3j} \\
&\text{Let } I=\int x^5\sqrt{ x^2+1}dx \\
&\text{Let } u=x^2+1, du=2xdx \\
&x^4=(x^2)^2=(u-1)^2 \\
&\begin{aligned}\\
\therefore I &=\frac{1}{2}\int(u-1)^2u^{1/2}du \\
&=\frac{1}{2}\int(u^{5/2}-2u^{3/2}+u^{1/2})du \\
&=\frac{1}{7}u^{7/2}-\frac{2}{5}u^{5/2}+\frac{1}{3}u^{3/2}+C \\
&=\frac{1}{7}(x^2+1)^{7/2}-\frac{2}{5}(x^2+1)^{5/2}+\frac{1}{3}(x^2+1)^{3/2}+C \\
\end{aligned}\\
&\text{3f} \\
&\text{Let }I=\int\frac{1}{\sqrt{ x^2+1 }}dx \\
&\text{Let }x=\tan \theta, \sqrt{ x^2+1}=\sec \theta \\
&dx=\sec^2d\theta \\
&\begin{aligned}\\
\therefore I&=\int\frac{\sec^2\theta d\theta}{\sec \theta} \\
&=\int \sec \theta d\theta \\
&=\ln|\sec \theta+\tan \theta|+C \\
&=\ln|x+\sqrt{ x^2+1 }|+C
\end{aligned} \\
&\text{3m} \\
&\int\frac{dx}{1+\cos x} \\
&=\frac{1}{2}\int\frac{2}{1+\cos x}dx \\
&=\int \frac{\sec^2x}{2}d(x/2) \\
&=\tan \frac{x}{2}+C \\
&\text{3k} \\
&\text{Let } I=\int \frac{1}{\sqrt{ 4x-x^2 }}dx=\int\frac{dx}{\sqrt{ 4-(x-2)^2 }} \\
&\text{Let }x-2=2\sin \theta \\
&\begin{aligned}\\
\sqrt{ 4x-x^2 }&=2\cos \theta \\
dx&=2\cos \theta d\theta \\
I&=\int\frac{2\cos \theta d\theta}{2\cos \theta}=\theta+C=\arcsin\frac{x-2}{2}+C
\end{aligned}\\
&\text{4a} \\
&\int xe^x dx \\
=&xe^x-\int e^xdx \\
=&xe^x-e^x+C \\
&\text{4c} \\
&\int x^2e^{-x}dx \\
=&-x^2e^{-x}-2xe^{-x}-2e^{-x}+c \\
&\text{4d} \\
&\int x \sin 3xdx \\
=&-\frac{1}{3}x\cos 3x + \frac{1}{9} \sin 3x +C \\
&\text{4e} \\
&\int 2x \sec^2 3x dx \\
=&\frac{2}{3} x \tan 3x -\frac{2}{9} \ln |\sec x|+C
\end{align}$$
# Whatever the fuck this is:
$$
\begin{align}
\int e^{3x}\cos 4xdx&=\frac{3}{25}e^{3x}\cos 4x+\frac{4}{25}e^{3x}\sin 4x +C\\
\int Re((A+Bi)e^{\alpha-i\beta})dx&=\int(Ae^{\alpha x}\cos \beta x+Be^{\alpha x}\sin \beta x)dx \\
\mathrm{Re}\left( (A+Bi) \int e^{(\alpha-i\beta)x}dx \right)&=\mathrm{Re} \left( \frac{A+Bi}{\alpha-i\beta}e^{(\alpha-i\beta)x} \right)+C \\
\mathrm{Re} (a+bi)&=a\\
\frac{1}{3-4i}&=\frac{3}{25}+\frac{4}{25}i \\ \\
&\text{1. }\int \frac{dx}{x-a}=\ln|x-a|+C \\
&\text{2. }\int \frac{(x-p)dx}{(x-p)^2+\xi^2}=\frac{1}{2}\ln((x-p)^2+\xi^2)+C \\
 &\text{3. }\int \frac{dx}{(x-p)^2+\xi^2}=\frac{1}{\xi}\tan^{-1} \frac{x-p}{\xi}+C
\end{align}
$$
